src/Analysis/Instances/Mixed/Int_Transfer.thy
@@ -376,7 +376,8 @@ definition int_tf_never_for :: "(vname => bool) => int_dom domain_transfer" wher
                             tf_return  = return_int_dom Refine_Never,
                             tf_enter   = enter_int_dom_for Refine_Never gs,
                             tf_event   = event_int_dom,
-                            tf_combine_env = combine_env_abs gs |)"
+                            tf_caller_cont = (\<lambda>_ \<sigma>. \<sigma>),
+                            tf_combine_env = (\<lambda>_. combine_env_abs gs) |)"
 
 definition int_tf_once_for :: "(vname => bool) => int_dom domain_transfer" where
   "int_tf_once_for gs = (| tf_assign  = assign_int_dom Refine_Once,
@@ -387,7 +388,8 @@ definition int_tf_once_for :: "(vname => bool) => int_dom domain_transfer" where
                            tf_return  = return_int_dom Refine_Once,
                            tf_enter   = enter_int_dom_for Refine_Once gs,
                            tf_event   = event_int_dom,
-                           tf_combine_env = combine_env_abs gs |)"
+                           tf_caller_cont = (\<lambda>_ \<sigma>. \<sigma>),
+                           tf_combine_env = (\<lambda>_. combine_env_abs gs) |)"
 
 definition int_tf_fixpoint_for :: "(vname => bool) => int_dom domain_transfer" where
   "int_tf_fixpoint_for gs = (| tf_assign  = assign_int_dom Refine_Fixpoint,
@@ -398,7 +400,8 @@ definition int_tf_fixpoint_for :: "(vname => bool) => int_dom domain_transfer" w
                                tf_return  = return_int_dom Refine_Fixpoint,
                                tf_enter   = enter_int_dom_for Refine_Fixpoint gs,
                                tf_event   = event_int_dom,
-                               tf_combine_env = combine_env_abs gs |)"
+                               tf_caller_cont = (\<lambda>_ \<sigma>. \<sigma>),
+                               tf_combine_env = (\<lambda>_. combine_env_abs gs) |)"
 
 lemma int_never_is_sound_transfer_for: "sound_transfer_for gs (int_tf_never_for gs)"
   unfolding int_tf_never_for_def
@@ -411,6 +414,7 @@ lemma int_never_is_sound_transfer_for: "sound_transfer_for gs (int_tf_never_for 
   subgoal by (simp add: return_int_dom_sound)
   subgoal by (simp add: enter_int_dom_for_sound)
   subgoal by (simp add: event_int_dom_sound)
+  subgoal by simp
   subgoal by (simp add: combine_env_sound)
   done
 
@@ -425,6 +429,7 @@ lemma int_once_is_sound_transfer_for: "sound_transfer_for gs (int_tf_once_for gs
   subgoal by (simp add: return_int_dom_sound)
   subgoal by (simp add: enter_int_dom_for_sound)
   subgoal by (simp add: event_int_dom_sound)
+  subgoal by simp
   subgoal by (simp add: combine_env_sound)
   done
 
@@ -439,6 +444,7 @@ lemma int_fixpoint_is_sound_transfer_for: "sound_transfer_for gs (int_tf_fixpoin
   subgoal by (simp add: return_int_dom_sound)
   subgoal by (simp add: enter_int_dom_for_sound)
   subgoal by (simp add: event_int_dom_sound)
+  subgoal by simp
   subgoal by (simp add: combine_env_sound)
   done
 
